src/Core/Solver/TD_Side/TD_Side_Eff_Cone_Lemmas.thy
@@ -509,13 +509,14 @@ lemma cone_compatible_etf_unit_transfer:
   fixes etf :: "(unit, 'a::sound_domain) effectful_domain_transfer"
     and F :: "edge_action \<Rightarrow> 'a abs_state \<Rightarrow> 'a abs_state"
     and Fe :: "vname list \<Rightarrow> exp list \<Rightarrow> 'a abs_state \<Rightarrow> 'a abs_state"
+    and Fc :: "vname option \<Rightarrow> 'a abs_state \<Rightarrow> 'a abs_state \<Rightarrow> 'a abs_state"
     and gs :: "vname \<Rightarrow> bool"
   assumes edge: "\<And>a u. apply_etf etf a u = unit_edge_tree gs (F a) u"
   assumes enter: "\<And>cl fs as. etf_enter etf fs as cl = unit_edge_tree gs (Fe fs as) cl"
-  assumes comb: "\<And>cc ex dst. etf_combine_collect etf dst cc ex = unit_combine_tree gs dst cc ex"
+  assumes comb: "\<And>cc ex dst. etf_combine_collect etf dst cc ex = unit_combine_tree gs (Fc dst) cc ex"
   shows "cone_compatible_etf gs etf"
 proof -
-  interpret mixed_rhs_generator gs etf F Fe
+  interpret mixed_rhs_generator gs etf Fc F Fe
     by (unfold_locales; simp add: edge enter comb)
   show ?thesis by (rule cone_compatible)
 qed
@@ -524,22 +525,27 @@ lemma threefold_mono_unit_transfer:
   fixes etf :: "(unit, 'a::sound_domain) effectful_domain_transfer"
     and F :: "edge_action \<Rightarrow> 'a abs_state \<Rightarrow> 'a abs_state"
     and Fe :: "vname list \<Rightarrow> exp list \<Rightarrow> 'a abs_state \<Rightarrow> 'a abs_state"
+    and Fc :: "vname option \<Rightarrow> 'a abs_state \<Rightarrow> 'a abs_state \<Rightarrow> 'a abs_state"
     and g :: cfg and bot0 s0 :: "'a abs_state" and gs :: "vname => bool"
   assumes edge: "\<And>a u. apply_etf etf a u = unit_edge_tree gs (F a) u"
   assumes enter: "\<And>cl fs as. etf_enter etf fs as cl = unit_edge_tree gs (Fe fs as) cl"
-  assumes comb: "\<And>cc ex dst. etf_combine_collect etf dst cc ex = unit_combine_tree gs dst cc ex"
+  assumes comb: "\<And>cc ex dst. etf_combine_collect etf dst cc ex = unit_combine_tree gs (Fc dst) cc ex"
   assumes mono: "\<And>a s1 s2. s1 \<le> s2 \<Longrightarrow> F a s1 \<le> F a s2"
   assumes mono_e: "\<And>fs as s1 s2. s1 \<le> s2 \<Longrightarrow> Fe fs as s1 \<le> Fe fs as s2"
+  assumes mono_c: "\<And>dst s1 s2 t1 t2. s1 \<le> s2 \<Longrightarrow> t1 \<le> t2 \<Longrightarrow> Fc dst s1 t1 \<le> Fc dst s2 t2"
   shows "threefold_mono (side_cfg_T_eff gs g etf bot0 s0 ())"
 proof -
-  interpret mixed_rhs_generator_mono gs etf F Fe
+  interpret mixed_rhs_generator_mono gs etf Fc F Fe
   proof unfold_locales
     show "\<And>a u. apply_etf etf a u = local_edge_tree gs (F a) u
                 \<or> apply_etf etf a u = unit_edge_tree gs (F a) u" by (simp add: edge)
     show "\<And>cl fs as. etf_enter etf fs as cl = unit_edge_tree gs (Fe fs as) cl" by (rule enter)
-    show "\<And>cc ex dst. etf_combine_collect etf dst cc ex = unit_combine_tree gs dst cc ex" by (rule comb)
+    show "\<And>cc ex dst. etf_combine_collect etf dst cc ex = unit_combine_tree gs (Fc dst) cc ex"
+      by (rule comb)
     show "\<And>a s1 s2. s1 \<le> s2 \<Longrightarrow> F a s1 \<le> F a s2" by (rule mono)
     show "\<And>fs as s1 s2. s1 \<le> s2 \<Longrightarrow> Fe fs as s1 \<le> Fe fs as s2" by (rule mono_e)
+    show "\<And>dst s1 s2 t1 t2. s1 \<le> s2 \<Longrightarrow> t1 \<le> t2 \<Longrightarrow> Fc dst s1 t1 \<le> Fc dst s2 t2"
+      by (rule mono_c)
   qed
   show ?thesis by (rule threefold_mono)
 qed
@@ -548,15 +554,16 @@ lemma cone_compatible_etf_local_unit_transfer:
   fixes etf :: "(unit, 'a::sound_domain) effectful_domain_transfer"
     and F :: "edge_action \<Rightarrow> 'a abs_state \<Rightarrow> 'a abs_state"
     and Fe :: "vname list \<Rightarrow> exp list \<Rightarrow> 'a abs_state \<Rightarrow> 'a abs_state"
+    and Fc :: "vname option \<Rightarrow> 'a abs_state \<Rightarrow> 'a abs_state \<Rightarrow> 'a abs_state"
     and gs :: "vname \<Rightarrow> bool"
   assumes edge: "\<And>a u. apply_etf etf a u =
     (if local_edge_action gs a then local_edge_tree gs (F a) u
      else unit_edge_tree gs (F a) u)"
   assumes enter: "\<And>cl fs as. etf_enter etf fs as cl = unit_edge_tree gs (Fe fs as) cl"
-  assumes comb: "\<And>cc ex dst. etf_combine_collect etf dst cc ex = unit_combine_tree gs dst cc ex"
+  assumes comb: "\<And>cc ex dst. etf_combine_collect etf dst cc ex = unit_combine_tree gs (Fc dst) cc ex"
   shows "cone_compatible_etf gs etf"
 proof -
-  interpret mixed_rhs_generator gs etf F Fe
+  interpret mixed_rhs_generator gs etf Fc F Fe
     by (unfold_locales; simp add: edge enter comb)
   show ?thesis by (rule cone_compatible)
 qed
@@ -565,24 +572,29 @@ lemma threefold_mono_local_unit_transfer:
   fixes etf :: "(unit, 'a::sound_domain) effectful_domain_transfer"
     and F :: "edge_action \<Rightarrow> 'a abs_state \<Rightarrow> 'a abs_state"
     and Fe :: "vname list \<Rightarrow> exp list \<Rightarrow> 'a abs_state \<Rightarrow> 'a abs_state"
+    and Fc :: "vname option \<Rightarrow> 'a abs_state \<Rightarrow> 'a abs_state \<Rightarrow> 'a abs_state"
     and g :: cfg and bot0 s0 :: "'a abs_state" and gs :: "vname => bool"
   assumes edge: "\<And>a u. apply_etf etf a u =
     (if local_edge_action gs a then local_edge_tree gs (F a) u
      else unit_edge_tree gs (F a) u)"
   assumes enter: "\<And>cl fs as. etf_enter etf fs as cl = unit_edge_tree gs (Fe fs as) cl"
-  assumes comb: "\<And>cc ex dst. etf_combine_collect etf dst cc ex = unit_combine_tree gs dst cc ex"
+  assumes comb: "\<And>cc ex dst. etf_combine_collect etf dst cc ex = unit_combine_tree gs (Fc dst) cc ex"
   assumes mono: "\<And>a s1 s2. s1 \<le> s2 \<Longrightarrow> F a s1 \<le> F a s2"
   assumes mono_e: "\<And>fs as s1 s2. s1 \<le> s2 \<Longrightarrow> Fe fs as s1 \<le> Fe fs as s2"
+  assumes mono_c: "\<And>dst s1 s2 t1 t2. s1 \<le> s2 \<Longrightarrow> t1 \<le> t2 \<Longrightarrow> Fc dst s1 t1 \<le> Fc dst s2 t2"
   shows "threefold_mono (side_cfg_T_eff gs g etf bot0 s0 ())"
 proof -
-  interpret mixed_rhs_generator_mono gs etf F Fe
+  interpret mixed_rhs_generator_mono gs etf Fc F Fe
   proof unfold_locales
     show "\<And>a u. apply_etf etf a u = local_edge_tree gs (F a) u
                 \<or> apply_etf etf a u = unit_edge_tree gs (F a) u" by (simp add: edge)
     show "\<And>cl fs as. etf_enter etf fs as cl = unit_edge_tree gs (Fe fs as) cl" by (rule enter)
-    show "\<And>cc ex dst. etf_combine_collect etf dst cc ex = unit_combine_tree gs dst cc ex" by (rule comb)
+    show "\<And>cc ex dst. etf_combine_collect etf dst cc ex = unit_combine_tree gs (Fc dst) cc ex"
+      by (rule comb)
     show "\<And>a s1 s2. s1 \<le> s2 \<Longrightarrow> F a s1 \<le> F a s2" by (rule mono)
     show "\<And>fs as s1 s2. s1 \<le> s2 \<Longrightarrow> Fe fs as s1 \<le> Fe fs as s2" by (rule mono_e)
+    show "\<And>dst s1 s2 t1 t2. s1 \<le> s2 \<Longrightarrow> t1 \<le> t2 \<Longrightarrow> Fc dst s1 t1 \<le> Fc dst s2 t2"
+      by (rule mono_c)
   qed
   show ?thesis by (rule threefold_mono)
 qed
@@ -602,15 +614,16 @@ lemma cone_compatible_etf_local_branch_unit_transfer:
     and F :: "edge_action \<Rightarrow> 'a abs_state \<Rightarrow> 'a abs_state"
     and Fe :: "vname list \<Rightarrow> exp list \<Rightarrow> 'a abs_state \<Rightarrow> 'a abs_state"
     and Fb :: "edge_action \<Rightarrow> 'a abs_state \<Rightarrow> 'a abs_state lifted"
+    and Fc :: "vname option \<Rightarrow> 'a abs_state \<Rightarrow> 'a abs_state \<Rightarrow> 'a abs_state"
     and gs :: "vname \<Rightarrow> bool"
   assumes edge: "\<And>a u. apply_etf etf a u = local_edge_tree gs (F a) u
       \<or> apply_etf etf a u = unit_edge_tree gs (F a) u
       \<or> apply_etf etf a u = local_branch_tree gs (Fb a) u"
   assumes enter: "\<And>cl fs as. etf_enter etf fs as cl = unit_edge_tree gs (Fe fs as) cl"
-  assumes comb: "\<And>cc ex dst. etf_combine_collect etf dst cc ex = unit_combine_tree gs dst cc ex"
+  assumes comb: "\<And>cc ex dst. etf_combine_collect etf dst cc ex = unit_combine_tree gs (Fc dst) cc ex"
   shows "cone_compatible_etf gs etf"
 proof -
-  interpret mixed_branch_rhs_generator gs etf F Fe Fb
+  interpret mixed_branch_rhs_generator gs etf Fc F Fe Fb
     by (unfold_locales; simp add: edge enter comb)
   show ?thesis by (rule cone_compatible)
 qed
@@ -620,29 +633,35 @@ lemma threefold_mono_local_branch_unit_transfer:
     and F :: "edge_action \<Rightarrow> 'a abs_state \<Rightarrow> 'a abs_state"
     and Fe :: "vname list \<Rightarrow> exp list \<Rightarrow> 'a abs_state \<Rightarrow> 'a abs_state"
     and Fb :: "edge_action \<Rightarrow> 'a abs_state \<Rightarrow> 'a abs_state lifted"
+    and Fc :: "vname option \<Rightarrow> 'a abs_state \<Rightarrow> 'a abs_state \<Rightarrow> 'a abs_state"
     and g :: cfg and bot0 s0 :: "'a abs_state" and gs :: "vname => bool"
   assumes edge: "\<And>a u. apply_etf etf a u = local_edge_tree gs (F a) u
       \<or> apply_etf etf a u = unit_edge_tree gs (F a) u
       \<or> apply_etf etf a u = local_branch_tree gs (Fb a) u"
   assumes enter: "\<And>cl fs as. etf_enter etf fs as cl = unit_edge_tree gs (Fe fs as) cl"
-  assumes comb: "\<And>cc ex dst. etf_combine_collect etf dst cc ex = unit_combine_tree gs dst cc ex"
+  assumes comb: "\<And>cc ex dst. etf_combine_collect etf dst cc ex = unit_combine_tree gs (Fc dst) cc ex"
   assumes mono: "\<And>a s1 s2. s1 \<le> s2 \<Longrightarrow> F a s1 \<le> F a s2"
   assumes mono_e: "\<And>fs as s1 s2. s1 \<le> s2 \<Longrightarrow> Fe fs as s1 \<le> Fe fs as s2"
   assumes mono_b: "\<And>a s1 s2. s1 \<le> s2 \<Longrightarrow> Fb a s1 \<le> Fb a s2"
+  assumes mono_c: "\<And>dst s1 s2 t1 t2. s1 \<le> s2 \<Longrightarrow> t1 \<le> t2 \<Longrightarrow> Fc dst s1 t1 \<le> Fc dst s2 t2"
   shows "threefold_mono (side_cfg_T_eff gs g etf bot0 s0 ())"
 proof -
-  interpret mixed_branch_rhs_generator_mono gs etf F Fe Fb
+  interpret mixed_branch_rhs_generator_mono gs etf Fc F Fe Fb
   proof unfold_locales
     show "\<And>a u. apply_etf etf a u = local_edge_tree gs (F a) u
                 \<or> apply_etf etf a u = unit_edge_tree gs (F a) u
                 \<or> apply_etf etf a u = local_branch_tree gs (Fb a) u" by (rule edge)
     show "\<And>cl fs as. etf_enter etf fs as cl = unit_edge_tree gs (Fe fs as) cl" by (rule enter)
-    show "\<And>cc ex dst. etf_combine_collect etf dst cc ex = unit_combine_tree gs dst cc ex" by (rule comb)
+    show "\<And>cc ex dst. etf_combine_collect etf dst cc ex = unit_combine_tree gs (Fc dst) cc ex"
+      by (rule comb)
     show "\<And>a s1 s2. s1 \<le> s2 \<Longrightarrow> F a s1 \<le> F a s2" by (rule mono)
     show "\<And>fs as s1 s2. s1 \<le> s2 \<Longrightarrow> Fe fs as s1 \<le> Fe fs as s2" by (rule mono_e)
     show "\<And>a s1 s2. s1 \<le> s2 \<Longrightarrow> Fb a s1 \<le> Fb a s2" by (rule mono_b)
+    show "\<And>dst s1 s2 t1 t2. s1 \<le> s2 \<Longrightarrow> t1 \<le> t2 \<Longrightarrow> Fc dst s1 t1 \<le> Fc dst s2 t2"
+      by (rule mono_c)
   qed
   show ?thesis by (rule threefold_mono)
 qed
+
 
 end
